Data -> Objectにリネーム res: 015

msgpack/Object.v
@@ -9,15 +9,15 @@ Fixpoint pow (m n : nat) :=
       m * pow m n'
   end.
 
-Inductive data :=
+Inductive object :=
 | Bool (_ : bool)
 | Nil
 | PFixnum: forall n,
-  nat_of_ascii n < 128 -> data
+  nat_of_ascii n < 128 -> object
 | NFixnum: forall n,
   (* 負の数を導入したくないので、補数表現を使う。 *)
   223 < nat_of_ascii n /\ nat_of_ascii n < 256 ->
-  data
+  object
 | Uint8  (_ : ascii)
 | Uint16 (_ _ : ascii)
 | Uint32 (_ _ _ _ : ascii)
@@ -29,54 +29,54 @@ Inductive data :=
 | Float  (_ _ _ _ : ascii)
 | Double (_ _ _ _ _ _ _ _ : ascii)
 | FixRaw: forall (xs : list ascii),
-  List.length xs < 32 -> data
+  List.length xs < 32 -> object
 | Raw16: forall (xs : list ascii),
-  List.length xs < pow 2 16 -> data
+  List.length xs < pow 2 16 -> object
 | Raw32: forall (xs : list ascii),
-  List.length xs < pow 2 32 -> data.
+  List.length xs < pow 2 32 -> object.
 
 (* データの等値性を定義。依存型の証明部分は無視する。*)
-Inductive eq_data : data -> data -> Prop :=
+Inductive eq_object : object -> object -> Prop :=
 | BoolEq : forall b,
-  eq_data (Bool b) (Bool b)
+  eq_object (Bool b) (Bool b)
 | NilEq  :
-  eq_data Nil Nil
+  eq_object Nil Nil
 | PFixnumEq: forall n m P Q,
   n = m ->
-  eq_data (PFixnum n P) (PFixnum m Q)
+  eq_object (PFixnum n P) (PFixnum m Q)
 | NFixnumEq: forall n m P Q,
   n = m ->
-  eq_data (NFixnum n P) (NFixnum m Q)
+  eq_object (NFixnum n P) (NFixnum m Q)
 | Uint8Eq : forall c,
-  eq_data (Uint8 c) (Uint8 c)
+  eq_object (Uint8 c) (Uint8 c)
 | Uint16Eq : forall c1 c2,
-  eq_data (Uint16 c1 c2) (Uint16 c1 c2)
+  eq_object (Uint16 c1 c2) (Uint16 c1 c2)
 | Uint32Eq : forall c1 c2 c3 c4,
-  eq_data (Uint32 c1 c2 c3 c4) (Uint32 c1 c2 c3 c4)
+  eq_object (Uint32 c1 c2 c3 c4) (Uint32 c1 c2 c3 c4)
 | Uint64Eq : forall c1 c2 c3 c4 c5 c6 c7 c8,
-  eq_data (Uint64 c1 c2 c3 c4 c5 c6 c7 c8) (Uint64 c1 c2 c3 c4 c5 c6 c7 c8)
+  eq_object (Uint64 c1 c2 c3 c4 c5 c6 c7 c8) (Uint64 c1 c2 c3 c4 c5 c6 c7 c8)
 | Int8Eq : forall c,
-  eq_data (Int8 c) (Int8 c)
+  eq_object (Int8 c) (Int8 c)
 | Int16Eq : forall c1 c2,
-  eq_data (Int16 c1 c2) (Int16 c1 c2)
+  eq_object (Int16 c1 c2) (Int16 c1 c2)
 | Int32Eq : forall c1 c2 c3 c4,
-  eq_data (Int32 c1 c2 c3 c4) (Int32 c1 c2 c3 c4)
+  eq_object (Int32 c1 c2 c3 c4) (Int32 c1 c2 c3 c4)
 | Int64Eq : forall c1 c2 c3 c4 c5 c6 c7 c8,
-  eq_data (Int64 c1 c2 c3 c4 c5 c6 c7 c8) (Int64 c1 c2 c3 c4 c5 c6 c7 c8)
+  eq_object (Int64 c1 c2 c3 c4 c5 c6 c7 c8) (Int64 c1 c2 c3 c4 c5 c6 c7 c8)
 | FloatEq : forall c1 c2 c3 c4,
-  eq_data (Float c1 c2 c3 c4) (Float c1 c2 c3 c4)
+  eq_object (Float c1 c2 c3 c4) (Float c1 c2 c3 c4)
 | DoubleEq : forall c1 c2 c3 c4 c5 c6 c7 c8,
-  eq_data (Double c1 c2 c3 c4 c5 c6 c7 c8) (Double c1 c2 c3 c4 c5 c6 c7 c8)
+  eq_object (Double c1 c2 c3 c4 c5 c6 c7 c8) (Double c1 c2 c3 c4 c5 c6 c7 c8)
 | FixRawEq : forall xs ys P Q,
-  eq_data (FixRaw xs P) (FixRaw ys Q)
+  eq_object (FixRaw xs P) (FixRaw ys Q)
 | Raw16Eq : forall xs ys P Q,
-  eq_data (Raw16 xs P) (Raw16 ys Q)
+  eq_object (Raw16 xs P) (Raw16 ys Q)
 | Raw32Eq : forall xs ys P Q,
-  eq_data (Raw32 xs P) (Raw32 ys Q).
+  eq_object (Raw32 xs P) (Raw32 ys Q).
 
-Infix "=~" := eq_data (at level 60, right associativity).
+Infix "=~" := eq_object (at level 60, right associativity).
 
-Ltac apply_data_eq :=
+Ltac apply_object_eq :=
   apply BoolEq    ||
   apply NilEq     ||
   apply PFixnumEq ||
@@ -100,7 +100,7 @@ Ltac apply_data_eq :=
 Lemma eq_sym : forall x,
   x =~ x.
 Proof.
-destruct x; apply_data_eq.
+destruct x; apply_object_eq.
  reflexivity.
 
  reflexivity.
@@ -110,7 +110,7 @@ Lemma eq_refl: forall x y,
   x =~ y -> y =~ x.
 Proof.
 intros.
-inversion H; apply_data_eq.
+inversion H; apply_object_eq.
  rewrite H0.
  reflexivity.
 
@@ -124,7 +124,7 @@ Proof.
 intros.
 inversion H;
   rewrite <- H2 in *; inversion H0;
-    apply_data_eq || (rewrite <- H3 in *; inversion H4);
+    apply_object_eq || (rewrite <- H3 in *; inversion H4);
     try inversion H5.
 
  rewrite H1, <- H3, <- H4 in *.
