msgpack/Soundness.v
@@ -1,17 +1,17 @@
-Require Import Data.
+Require Import Object.
 Require Import Serialize.
 
-Theorem recover: forall data1 bytes data2,
-  Serialized data1 bytes ->
-  Serialized data2 bytes ->
-  data1 =~ data2.
+Theorem recover: forall object1 bytes object2,
+  Serialized object1 bytes ->
+  Serialized object2 bytes ->
+  object1 =~ object2.
 Proof.
 intros.
 inversion H;
   rewrite <- H2 in *;
   clear H2;
   inversion H0;
-  apply_data_eq.
+  apply_object_eq.
 
  rewrite H5,H6,H7,H8,H9,H10.
  tauto.
